Fixes to notations, warnings, and Makefile.

progs/threads.c
@@ -24,6 +24,11 @@ void release(void *lock) {
   return;
 }
 
+void makelock2(void *lock) {
+  pthread_mutex_init((pthread_mutex_t*)lock, NULL);
+  pthread_mutex_lock((pthread_mutex_t*)lock);
+}
+
 void freelock2(void *lock) {
   pthread_mutex_destroy((pthread_mutex_t*)lock);
   return;
