Makefile
@@ -514,7 +514,8 @@ aes: _CoqProject $(AES_FILES:%.v=aes/%.vo)
 hkdf:    _CoqProject $(HKDF_FILES:%.v=sha/%.vo)
 # drbg: _CoqProject $(DRBG_FILES:%.v=verifiedDrbg/%.vo)
 mailbox: _CoqProject mailbox/verif_mailbox_all.vo
-atomics: _CoqProject atomics/verif_kvnode_atomic.vo atomics/verif_kvnode_atomic_ra.vo atomics/verif_hashtable_atomic.vo atomics/verif_hashtable_atomic_ra.vo
+#atomics: _CoqProject atomics/verif_kvnode_atomic.vo atomics/verif_kvnode_atomic_ra.vo atomics/verif_hashtable_atomic.vo atomics/verif_hashtable_atomic_ra.vo atomics/general_locks.vo
+atomics: _CoqProject atomics/verif_hashtable_atomic.vo progs/verif_incr_atomic.vo
 io: _CoqProject progs/verif_printf.vo progs/verif_io.vo progs/verif_io_mem.vo
 
 CGFLAGS =  -DCOMPCERT
